Lean/Geo/KGon/Assn.lean
@@ -9,28 +9,28 @@ namespace Geo.CanonicalPoints
 open List Classical LeanSAT.Model PropFun Point
 attribute [-simp] getElem_fin
 
-def isCap (w : CanonicalPoints) (a c d : Fin w.length) (o : Orientation) :=
+def isCap (w : CanonicalPoints) (a c d : Fin w.rlen) (o : Orientation) :=
   ∃ b, a < b ∧ b < c ∧ c < d ∧
-    σ w[a] w[b] w[c] = o ∧ σ w[b] w[c] w[d] = o
+    σ w+[a] w+[b] w+[c] = o ∧ σ w+[b] w+[c] w+[d] = o
 
-def isCapF (w : CanonicalPoints) (a c d : Fin w.length) :=
-  c < d ∧ ∃ b : Fin w.length, isCap w a b c .cw ∧
-    σ w[b] w[c] w[d] = .cw ∧ σIsEmptyTriangleFor w[a] w[b] w[d] w.toFinset
+def isCapF (w : CanonicalPoints) (a c d : Fin w.rlen) :=
+  c < d ∧ ∃ b : Fin w.rlen, isCap w a b c .cw ∧
+    σ w+[b] w+[c] w+[d] = .cw ∧ σIsEmptyTriangleFor w+[a] w+[b] w+[d] w.toFinset
 
-@[simp] def toPropAssn (w : CanonicalPoints) : Var w.length → Prop
-  | .sigma a b c    => σ w[a] w[b] w[c] = .ccw
-  | .inside x a b c => σPtInTriangle w[x] w[a] w[b] w[c]
-  | .hole a b c     => σIsEmptyTriangleFor w[a] w[b] w[c] w.toFinset
+@[simp] def toPropAssn (w : CanonicalPoints) : Var w.rlen → Prop
+  | .sigma a b c    => σ w+[a] w+[b] w+[c] = .ccw
+  | .inside x a b c => σPtInTriangle w+[x] w+[a] w+[b] w+[c]
+  | .hole a b c     => σIsEmptyTriangleFor w+[a] w+[b] w+[c] w.toFinset
   | .cap a c d      => isCap w a c d .cw
   | .cup a c d      => isCap w a c d .ccw
   | .capF a d e     => isCapF w a d e
 
 theorem satisfies_signotopeClauses (w : CanonicalPoints) :
-    (signotopeClauses w.length).eval w.toPropAssn := by
+    (signotopeClauses w.rlen).eval w.toPropAssn := by
   simp [signotopeClauses]
-  intro i _ j hij k hjk l hkl
-  have s : Sorted₄ w[i] w[j] w[k] w[l] := w.sorted₄ hij hjk hkl
-  have gp : InGeneralPosition₄ w[i] w[j] w[k] w[l] := w.gp₄ hij hjk hkl
+  intro i j hij k hjk l hkl
+  have s := w.sorted₄' hij hjk hkl
+  have gp := w.gp₄' hij hjk hkl
   constructor
   . exact σ_prop₂ s gp
   -- constructor
@@ -69,62 +69,55 @@ theorem insideDefs_aux₂ {a b x c : Point} : Sorted₄ a b x c → InGeneralPos
     rw [σ_prop₃ sorted gp h₁ h₄] at h₃
     contradiction
 
-theorem satisfies_insideClauses (w : CanonicalPoints) : (insideClauses w.length).eval w.toPropAssn := by
+theorem satisfies_insideClauses (w : CanonicalPoints) : (insideClauses w.rlen).eval w.toPropAssn := by
   simp [insideClauses]
-  intro a _ b hab c hbc x
+  intro a b hab c hbc x
   constructor
   · intro hax hxb
-    exact (insideDefs_aux₁ (w.sorted₄ hax hxb hbc) (w.gp₄ hax hxb hbc)).1
+    exact (insideDefs_aux₁ (w.sorted₄' hax hxb hbc) (w.gp₄' hax hxb hbc)).1
   · intro hbx hxc
-    exact (insideDefs_aux₂ (w.sorted₄ hab hbx hxc) (w.gp₄ hab hbx hxc)).1
+    exact (insideDefs_aux₂ (w.sorted₄' hab hbx hxc) (w.gp₄' hab hbx hxc)).1
 
-theorem satisfies_holeDefClauses (w : CanonicalPoints) : (holeDefClauses w.length).eval w.toPropAssn := by
+theorem satisfies_holeDefClauses (w : CanonicalPoints) : (holeDefClauses w.rlen).eval w.toPropAssn := by
   simp [holeDefClauses, σIsEmptyTriangleFor, mem_toFinset_iff]
-  intro a _ b ab c bc H i tri
-  have gp₄ : InGeneralPosition₄ w[i] w[a] w[b] w[c] := tri.gp₄_of_gp₃ (w.gp₃ ab bc)
-  have ib : i ≠ b := mt (congrArg (w[·])) gp₄.gp₃.ne₁
-  have ⟨wawi, wiwc⟩ := xBounded_of_PtInTriangle' (w.sorted₃ ab bc) ((σPtInTriangle_iff gp₄).mp tri)
-  have ai : a < i := w.lt_iff.1 <| by
+  intro a b ab c bc H i tri
+  have gp₄ : InGeneralPosition₄ w[i] w+[a] w+[b] w+[c] := tri.gp₄_of_gp₃ (w.gp₃' ab bc)
+  have ib : i ≠ b.succ := mt (congrArg (w[·])) gp₄.gp₃.ne₁
+  have ⟨wawi, wiwc⟩ := xBounded_of_PtInTriangle' (w.sorted₃' ab bc) ((σPtInTriangle_iff gp₄).mp tri)
+  have ai : a.succ < i := w.lt_iff.1 <| by
     apply lt_of_le_of_ne wawi
     intro h
     exact gp₄.gp₁.ne₁ <| w.eq_iff.1 h.symm ▸ rfl
-  have ic : i < c := w.lt_iff.1 <| by
+  have ic : i < c.succ := w.lt_iff.1 <| by
     apply lt_of_le_of_ne wiwc
     intro h
     exact gp₄.gp₃.ne₂ <| w.eq_iff.1 h ▸ rfl
-  exact H i ai ic ib tri
-
-theorem satisfies_leftmostCCWDefs (w : CanonicalPoints) :
-    (leftmostCCWClauses w.length).eval w.toPropAssn := by
-  simp [leftmostCCWClauses]
-  intro i h0i j hij
-  let ⟨i+1, hi⟩ := i; let ⟨j+1, hj⟩ := j
-  exact List.pairwise_iff_get.1 w.oriented
-    ⟨_, Nat.lt_of_succ_lt_succ hi⟩ ⟨_, Nat.lt_of_succ_lt_succ hj⟩ (Nat.lt_of_succ_lt_succ hij)
+  obtain rfl | ⟨i,rfl⟩ := i.eq_zero_or_eq_succ
+  · cases ai
+  · exact H i (Fin.succ_lt_succ_iff.1 ai) (Fin.succ_lt_succ_iff.1 ic) (mt Fin.succ_inj.2 ib) tri
 
 theorem satisfies_revLexClausesCore {F : Fin n → _} {F' : Fin m → _}
-    (hF : ∀ a a', a'.1 = a.1 + 1 → ((F' a').eval τ ↔ F a))
-    (ha : a'.1 = a.1 + 1) (hb : b'.1 = b.1 + 1) (hacc : acc → acc'.eval τ) :
+    (hF : ∀ a a', a'.1 = a.1 → ((F' a').eval τ ↔ F a))
+    (ha : a'.1 = a.1) (hb : b'.1 = b.1) (hacc : acc → acc'.eval τ) :
     RevLexMid F a b acc → (revLexClausesCore (α := α) F' a' b' acc').eval τ := by
   unfold RevLexMid revLexClausesCore
   have : a' < b' ↔ a < b := by simp [Fin.lt_def, -Fin.val_fin_lt, ha, hb]
   simp [this]; split
   · apply satisfies_revLexClausesCore hF <;> simp [ha, hb]
-    · rw [Fin.lt_def] at *; omega
-    · simp [hF _ _ ha, hF _ _ hb]
-      exact .imp_right <| .imp_right hacc
+    simp [hF _ _ ha, hF _ _ hb]
+    exact .imp_right <| .imp_right hacc
   · exact hacc
 
-theorem satisfies_revLexClauses (w : CanonicalPoints) : (revLexClauses w.length).eval w.toPropAssn := by
+theorem satisfies_revLexClauses (w : CanonicalPoints) : (revLexClauses w.rlen).eval w.toPropAssn := by
   simp [revLexClauses, length, points]
-  intro h5w
+  intro h4w
   have := w.lex (by omega)
   simp [σRevLex, RevLexMid3] at this
-  refine satisfies_revLexClausesCore ?_ (by simp) (by simp; omega) (by simp) this
+  refine satisfies_revLexClausesCore ?_ rfl rfl (by simp) this
   rintro ⟨a, ha⟩ ⟨_, ha'⟩ ⟨⟩; simp [getElem, points]
 
-theorem satisfies_baseEncoding (w : CanonicalPoints) : (baseEncoding w.length).eval w.toPropAssn := by
+theorem satisfies_baseEncoding (w : CanonicalPoints) : (baseEncoding w.rlen).eval w.toPropAssn := by
   simp [baseEncoding, satisfies_signotopeClauses, satisfies_insideClauses, satisfies_holeDefClauses,
-    satisfies_leftmostCCWDefs, satisfies_revLexClauses]
+    satisfies_revLexClauses]
 
 end CanonicalPoints
