Lean/Geo/Hexagon/Assn.lean
@@ -11,83 +11,86 @@ namespace Geo.CanonicalPoints
 open List Classical LeanSAT.Model PropFun Point
 attribute [-simp] getElem_fin
 
-theorem satisfies_capDef (w : CanonicalPoints) {a b c d : Fin (length w)}
+theorem satisfies_capDef (w : CanonicalPoints) {a b c d : Fin w.rlen}
     (ab : a < b) (bc : b < c) (cd : c < d) : (capDef a b c d).eval w.toPropAssn := by
   simp [capDef, isCap]; intro h1 h2
-  exact ⟨_, ab, bc, cd, (w.gp₃ ab bc).σ_iff.1 h1, (w.gp₃ bc cd).σ_iff.1 h2⟩
+  exact ⟨_, ab, bc, cd, (w.gp₃' ab bc).σ_iff.1 h1, (w.gp₃' bc cd).σ_iff.1 h2⟩
 
-theorem satisfies_capDef2 (w : CanonicalPoints) {a c d : Fin (length w)} :
+theorem satisfies_capDef2 (w : CanonicalPoints) {a c d : Fin w.rlen} :
     (capDef2 a c d).eval w.toPropAssn := by
   simp [capDef2, isCap]; intro b ab bc cd h1 h2
-  have gp := w.gp₄ ab bc cd
-  exact gp.gp₃.σ_iff.2 <| σ_prop₃ (w.sorted₄ ab bc cd) gp h1 h2
+  have gp := w.gp₄' ab bc cd
+  exact gp.gp₃.σ_iff.2 <| σ_prop₃ (w.sorted₄' ab bc cd) gp h1 h2
 
-theorem satisfies_cupDef (w : CanonicalPoints) {a b c d : Fin (length w)}
+theorem satisfies_cupDef (w : CanonicalPoints) {a b c d : Fin w.rlen}
     (ab : a < b) (bc : b < c) (cd : c < d) : (cupDef a b c d).eval w.toPropAssn := by
   simp [cupDef, isCap]; intro h1 h2
   exact ⟨_, ab, bc, cd, h1, h2⟩
 
-theorem satisfies_cupDef2 (w : CanonicalPoints) {a c d : Fin (length w)} :
+theorem satisfies_cupDef2 (w : CanonicalPoints) {a c d : Fin w.rlen} :
     (cupDef2 a c d).eval w.toPropAssn := by
   simp [cupDef2, isCap]; intro b ab bc cd h1 h2
-  exact σ_prop₁ (w.sorted₄ ab bc cd) (w.gp₄ ab bc cd) h1 h2
+  exact σ_prop₁ (w.sorted₄' ab bc cd) (w.gp₄' ab bc cd) h1 h2
 
-theorem satisfies_capFDef (w : CanonicalPoints) {a b c d : Fin (length w)} (bc : b < c) (cd : c < d)
-    (hh : σIsEmptyTriangleFor w[a] w[b] w[d] w.toFinset) : (capFDef a b c d).eval w.toPropAssn := by
+theorem satisfies_capFDef (w : CanonicalPoints) {a b c d : Fin w.rlen} (bc : b < c) (cd : c < d)
+    (hh : σIsEmptyTriangleFor w+[a] w+[b] w+[d] w.toFinset) :
+    (capFDef a b c d).eval w.toPropAssn := by
   simp [capFDef, isCapF]; intro h1 h2
-  exact ⟨cd, _, h2, (w.gp₃ bc cd).σ_iff.1 h1, hh⟩
+  exact ⟨cd, _, h2, (w.gp₃' bc cd).σ_iff.1 h1, hh⟩
 
 theorem satisfies_no6Hole3Below {w : CanonicalPoints} (hw : ¬σHasEmptyKGon 6 w.toFinset)
-    {a c d e : Fin (length w)} (ha : 0 < a) (de : d < e)
-    (ace : σIsEmptyTriangleFor w[a] w[c] w[e] w.toFinset) :
+    {a c d e : Fin w.rlen} (de : d < e)
+    (ace : σIsEmptyTriangleFor w+[a] w+[c] w+[e] w.toFinset) :
     (no6Hole3Below a c d e).eval w.toPropAssn := by
   simp [no6Hole3Below]; intro ⟨b, ab, bc, cd, abc, bcd⟩ cde
-  refine hw <| σCCWPoints.emptyHexagon' ?_ w.gp ace (subset_map w [0, a, b, c, d, e])
-  exact Arc.join (l₁ := [a,b,c,d]) (l₂ := [])
-    (.cons ha (w.σ_0 ha ab) <| .cons ab abc <| .cons bc bcd <| .cons cd cde <| .one de)
-    (.one <| ha.trans <| ab.trans <| bc.trans <| cd.trans de)
+  refine hw <| σCCWPoints.emptyHexagon' ?_ w.gp ace
+    (subset_map w [0, a.succ, b.succ, c.succ, d.succ, e.succ])
+  exact Arc.join (l₁ := [_,_,_,_]) (l₂ := [])
+    (.cons (Fin.succ_pos _) (w.σ_0 ab) <|
+      .cons' ab abc <| .cons' bc bcd <| .cons' cd cde <| .one' de)
+    (.one <| Fin.succ_pos _)
 
 theorem satisfies_no6Hole4Above {w : CanonicalPoints} (hw : ¬σHasEmptyKGon 6 w.toFinset)
-    {a d e f : Fin (length w)} (ef : e < f) :
+    {a d e f : Fin w.rlen} (ef : e < f) :
     (no6Hole4Above a d e f).eval w.toPropAssn := by
   simp [no6Hole4Above]; intro ⟨de, c, ⟨b, ab, bc, cd, abc, bcd⟩, cde, ace⟩
-  refine (w.gp₃ de ef).σ_iff'.1 fun def_ => ?_
+  refine (w.gp₃' de ef).σ_iff'.1 fun def_ => ?_
   refine hw <| (σCCWPoints.cycle (l₂ := [_, _, _, _, _]) ?_).emptyHexagon'
-    w.gp ace.perm₂.perm₁.perm₂ (subset_map w [f, e, d, c, b, a])
-  exact Arc.join (l₁ := []) (l₂ := [b,c,d,e])
-    (.one <| ab.trans <| bc.trans <| cd.trans <| de.trans ef)
-    (.cons ab abc <| .cons bc bcd <| .cons cd cde <| .cons de def_ <| .one ef)
+    w.gp ace.perm₂.perm₁.perm₂ (subset_map' w [f, e, d, c, b, a])
+  exact Arc.join (l₁ := []) (l₂ := [_,_,_,_])
+    (.one' <| ab.trans <| bc.trans <| cd.trans <| de.trans ef)
+    (.cons' ab abc <| .cons' bc bcd <| .cons' cd cde <| .cons' de def_ <| .one' ef)
 
 theorem satisfies_no6Hole2Below {w : CanonicalPoints} (hw : ¬σHasEmptyKGon 6 w.toFinset)
-    {a c e f : Fin (length w)} :
+    {a c e f : Fin w.rlen} :
     (no6Hole2Below a c f e).eval w.toPropAssn := by
   simp [no6Hole2Below]; intro ⟨b, ab, bc, cf, abc, bcd⟩ ⟨d, ad, de, ef, ade, def_⟩ hh
-  have := Arc.join (l₁ := [b,c]) (l₂ := [d,e])
-    (.cons ab abc <| .cons bc bcd <| .one cf)
-    (.cons ad ade <| .cons de def_ <| .one ef)
-  refine hw <| this.emptyHexagon w.gp ?_ (subset_map w [a, b, c, f, e, d])
+  have := Arc.join (l₁ := [_,_]) (l₂ := [_,_])
+    (.cons' ab abc <| .cons' bc bcd <| .one' cf)
+    (.cons' ad ade <| .cons' de def_ <| .one' ef)
+  refine hw <| this.emptyHexagon w.gp ?_ (subset_map' w [a, b, c, f, e, d])
   split_ifs at hh with ce <;> simp at hh <;> [exact hh; exact hh.perm₂]
 
 theorem satisfies_no6Hole1Below {w : CanonicalPoints} (hw : ¬σHasEmptyKGon 6 w.toFinset)
-    {a d e f : Fin (length w)} (ae : a < e) (ef : e < f) :
+    {a d e f : Fin w.rlen} (ae : a < e) (ef : e < f) :
     (no6Hole1Below a d f e).eval w.toPropAssn := by
   simp [no6Hole1Below]; intro ⟨df, c, ⟨b, ab, bc, cd, abc, bcd⟩, cdf, acf⟩ aef
-  have := Arc.join (l₁ := [e]) (l₂ := [b,c,d])
-    (.cons ae aef <| .one ef)
-    (.cons ab abc <| .cons bc bcd <| .cons cd cdf <| .one df)
-  refine hw <| this.emptyHexagon w.gp acf.perm₂ (subset_map w [a, e, f, d, c, b])
+  have := Arc.join (l₁ := [_]) (l₂ := [_,_,_])
+    (.cons' ae aef <| .one' ef)
+    (.cons' ab abc <| .cons' bc bcd <| .cons' cd cdf <| .one' df)
+  refine hw <| this.emptyHexagon w.gp acf.perm₂ (subset_map' w [a, e, f, d, c, b])
 
 theorem satisfies_hexagonEncoding (w : CanonicalPoints) (hw : ¬σHasEmptyKGon 6 w.toFinset) :
-    (hexagonEncoding w.length).eval w.toPropAssn := by
+    (hexagonEncoding w.rlen).eval w.toPropAssn := by
   simp [hexagonEncoding, satisfies_baseEncoding, no6HoleClauses1, no6HoleClauses2, no6HoleClauses3]
   refine ⟨
-    fun a ha b ab c bc d cd => ⟨?_, ?_, fun _ => ⟨fun hh => ⟨?_, ?_⟩, fun _ => ?_⟩⟩,
-    fun a _ b _ c _ => ⟨?_, ?_⟩,
-    fun a _ b _ c _ p ap pc _ => ⟨fun _ _ => ?_, fun _ => ?_⟩⟩
+    fun a b ab c bc d cd => ⟨?_, ?_, fun _ => ⟨fun hh => ⟨?_, ?_⟩, fun _ => ?_⟩⟩,
+    fun a b _ c _ => ⟨?_, ?_⟩,
+    fun a b _ c _ p ap pc _ => ⟨fun _ _ => ?_, fun _ => ?_⟩⟩
   · with_reducible exact satisfies_capDef w ab bc cd
   · with_reducible exact satisfies_cupDef w ab bc cd
   · with_reducible exact satisfies_capFDef w bc cd hh
-  · with_reducible exact satisfies_no6Hole3Below hw ha cd hh
+  · with_reducible exact satisfies_no6Hole3Below hw cd hh
   · with_reducible exact satisfies_no6Hole4Above hw cd
   · with_reducible exact satisfies_capDef2 w
   · with_reducible exact satisfies_cupDef2 w
