Lean/Geo/Triangle/RunEncoding.lean
@@ -9,9 +9,9 @@ def main (args : List String) : IO Unit := do
   match args with
   | [] => IO.println "expected one argument (number of points)"
   | n::rest =>
-  let some n := String.toNat? n
+  let some (rlen + 1) := String.toNat? n
     | throw (.userError "hi")
-  let (vars, enc) := Geo.triangleEncoding n |>.toICnf compare
+  let (vars, enc) := Geo.triangleEncoding rlen |>.toICnf compare
   if let out::_ := rest then
     let h ← IO.FS.Handle.mk out IO.FS.Mode.write
     for v in vars do
